rustfrontend/Rusttypes.v
@@ -60,6 +60,22 @@ Proof.
 Defined.  
 
 
+Inductive variance :=
+| Covariant
+| Invariant.
+
+Lemma variance_eq: forall (va1 va2: variance), {va1 = va2} + {va1 <> va2}.
+decide equality.
+Defined.
+
+Definition join_variance (v1 v2: variance) :=
+  match v1, v2 with
+  | Invariant, _
+  | _, Invariant => Invariant
+  | _, _ => Covariant
+  end.
+
+
 (** ** Types  *)
 
 Inductive type : Type :=
